Fifo/GenericProofs.v
@@ -8,27 +8,84 @@ Require Import StdLibKami.Fifo.Ifc.
 Require Import StdLibKami.Fifo.GenericSpec.
 Require Import StdLibKami.Fifo.DoubleFifo.
 Require Import StdLibKami.Fifo.CorrectDef.
+Require Import StdLibKami.Fifo.Proofs2.
 
+
+Definition valsToSnd {k : Kind} (l : list (type k)) :=
+  map (fun x => existT (fullType type) (SyntaxKind k)
+                       (nth_default (evalConstT Default) l x)) (seq 0 (length l)).
 
 Section Proofs.
-  Context {ifcParams' : Fifo.Ifc.Params}.
-  Context {dblParams' : Fifo.DoubleFifo.Params}.
-  
-  Local Definition fifoImpl1 := @Fifo.DoubleFifo.impl ifcParams' dblParams'.
-  Local Definition fifoImpl2 := @Fifo.GenericSpec.spec ifcParams'.
+  Context {ifcParams : Fifo.Ifc.Params}.
+  Context {dblParams : Fifo.DoubleFifo.Params}.
 
-  Record myFifoImpl1R  (implRegs : RegsT) (fifo1_bval : bool) (fifo1_dval : type k)
-         (o_i o_s : RegsT) : Prop :=
+  Local Definition fifoImpl := @Fifo.DoubleFifo.impl ifcParams dblParams.
+  Local Definition fifoSpec := @Fifo.GenericSpec.spec ifcParams.
+  Local Definition fifoSpecL := @Fifo.GenericSpec.spec (@Fifo.DoubleFifo.ifcParamsL ifcParams).
+  Local Definition fifoSpecR := @Fifo.GenericSpec.spec (@Fifo.DoubleFifo.ifcParamsR ifcParams).
+  
+  Variable HCorrectL : FifoCorrect Lfifo fifoSpecL.
+  Variable HCorrectR : FifoCorrect Rfifo fifoSpecR.
+  
+  Record myGenFifoR  (o_i o_s : RegsT) : Prop :=
     {
-      implRegVal : implRegs = [(Fifo1.validRegName,
-                                existT _ (SyntaxKind Bool) fifo1_bval);
-                              (Fifo1.dataRegName,
-                               existT _ (SyntaxKind k) fifo1_dval)];
-      Ho_iCorrect1 : o_i = implRegs;
-      Ho_sCorrect1 : o_s = implRegs;
+      o_i1 : RegsT;
+      o_i2 : RegsT;
+      o_s1 : RegsT;
+      o_s2 : RegsT;
+      implRegsL : RegsT;
+      implRegsR : RegsT;
+      implRegValL : list (type k);
+      implRegValR : list (type k);
+      specRegVals : list (type k);
+      nonDetEmpVal : bool;
+      nonDetEmpValL : bool;
+      lenVal : word lgSize;
+      lenValL : word (@lgSize (@Fifo.DoubleFifo.ifcParamsL ifcParams));
+      lenValR : word (@lgSize (@Fifo.DoubleFifo.ifcParamsR ifcParams));
+      HimplRegValL : specRegVals = implRegValL ++ implRegValR;
+      HnonDetEmpVal : nonDetEmpVal = nonDetEmpValL;
+      Ho_sCorrect : o_s =
+                    [(GenericSpec.nonDetEmptyName, existT _ (SyntaxKind Bool) nonDetEmpVal);
+                    (GenericSpec.listName, existT _ (GenericSpec.nlist type) specRegVals);
+                    (GenericSpec.nonDetLenName, existT _ (SyntaxKind (Bit lgSize)) lenVal)];
+      Ho_s1Correct : o_s1 =
+                    [((@GenericSpec.nonDetEmptyName (@Fifo.DoubleFifo.ifcParamsL ifcParams)), existT _ (SyntaxKind Bool) nonDetEmpVal);
+                    ((@GenericSpec.listName (@Fifo.DoubleFifo.ifcParamsL ifcParams)), existT _ (GenericSpec.nlist type) specRegVals);
+                    ((@GenericSpec.nonDetLenName (@Fifo.DoubleFifo.ifcParamsL ifcParams)), existT _ (SyntaxKind (Bit lgSize)) lenVal)];
+      Ho_iApp : o_i = o_i1 ++ o_i2;
+      HRegs1 : getKindAttr o_i1 = (fifoRegs HCorrectL);
+      HRegs2 : getKindAttr o_i2 = (fifoRegs HCorrectR);
+      HfifoR1 : (fifoR HCorrectL) o_i1 o_s1;
+      HfifoR2 : (fifoR HCorrectR) o_i2 o_s2;
       Ho_iNoDup1 : NoDup (map fst o_i);
       Ho_sNoDup1 : NoDup (map fst o_s);
     }.
 
+  Ltac Record_destruct :=
+    match goal with
+    | [H : myGenFifoR _ _ |- _] =>
+      destruct H
+    end.
+
+  Goal FifoCorrect fifoImpl fifoSpec.
+    destruct HCorrectL, HCorrectR.
+    econstructor 1 with (fifoR := myGenFifoR)
+                        (fifoRegs := fifoRegs ++ fifoRegs0).
+    all : unfold EffectfulRelation, EffectlessRelation,
+          fifoImpl, fifoSpec, impl, spec,
+          isEmpty, isFull, numFree, first, deq, enq, flush,
+          GenericSpec.isEmpty, GenericSpec.isFull, GenericSpec.numFree, GenericSpec.first,
+          GenericSpec.deq, GenericSpec.enq, GenericSpec.flush,
+          DoubleFifo.isEmpty, DoubleFifo.isFull, DoubleFifo.numFree, DoubleFifo.first,
+          DoubleFifo.deq, DoubleFifo.enq, DoubleFifo.flush.
+    all: intros; try Record_destruct; destruct HCorrectL, HCorrectR;
+      cbn [CorrectDef.fifoRegs CorrectDef.fifoR] in *.
+    - unfold fifoSpecL, spec, GenericSpec.isEmpty, GenericSpec.numFree in *; cbn [isEmpty] in *.
+      hyp_consumer.
+      goal_consumer1.
+      unfold GenericSpec.nlist, DoubleFifo.ifcParamsL, k in x1.
+      rewrite (Eqdep.EqdepTheory.UIP_refl _ _ x1).
+  Admitted.
   
 End Proofs.
